Empty.v goes through

theories/Substitution/Introductions/Empty.v
@@ -1,7 +1,7 @@
 From LogRel.AutoSubst Require Import core unscoped Ast Extra.
-From LogRel Require Import Utils BasicAst Notations Context NormalForms Weakening GenericTyping LogicalRelation Validity.
-From LogRel.LogicalRelation Require Import Induction Irrelevance Escape Reflexivity Weakening Neutral Transitivity Reduction Application Universe SimpleArr.
-From LogRel.Substitution Require Import Irrelevance Properties Conversion SingleSubst Reflexivity.
+From LogRel Require Import Utils BasicAst Notations LContexts Context NormalForms Weakening GenericTyping LogicalRelation Monad Validity.
+From LogRel.LogicalRelation Require Import Induction Irrelevance Escape Reflexivity Weakening Monotonicity Split Neutral Transitivity Reduction Application Universe SimpleArr.
+From LogRel.Substitution Require Import Irrelevance Properties Conversion SingleSubst Reflexivity Monotonicity.
 From LogRel.Substitution.Introductions Require Import Universe Pi SimpleArr Var.
 
 Set Universe Polymorphism.
@@ -12,33 +12,40 @@ Context `{GenericTypingProperties}.
 Set Printing Primitive Projection Parameters.
 
 
-Lemma emptyRed {Γ l} : [|- Γ] -> [Γ ||-<l> tEmpty].
+Lemma emptyRed {wl Γ l} : [|- Γ]< wl > -> [Γ ||-<l> tEmpty]< wl >.
 Proof. 
   intros; eapply LREmpty_; constructor; eapply redtywf_refl; gen_typing.
 Defined.
 
-Lemma emptyValid {Γ l} (VΓ : [||-v Γ]) : [Γ ||-v<l> tEmpty | VΓ].
+
+Lemma emptyValid {wl Γ l} (VΓ : [||-v Γ]< wl >) : [Γ ||-v<l> tEmpty | VΓ]< wl >.
 Proof.
   unshelve econstructor; intros.
-  + now eapply emptyRed.
-  + cbn; constructor; eapply redtywf_refl; gen_typing.
+  + now eapply LogtoW, emptyRed.
+  + eapply EqLogtoW.
+    cbn; constructor; eapply redtywf_refl; gen_typing.
 Defined.
 
-Lemma emptyconvValid {Γ l} (VΓ : [||-v Γ]) (VEmpty : [Γ ||-v<l> tEmpty | VΓ]) : 
-  [Γ ||-v<l> tEmpty ≅ tEmpty | VΓ | VEmpty].
+
+Lemma emptyconvValid {wl Γ l} (VΓ : [||-v Γ]< wl >) (VEmpty : [Γ ||-v<l> tEmpty | VΓ]< wl >) : 
+  [Γ ||-v<l> tEmpty ≅ tEmpty | VΓ | VEmpty]< wl >.
 Proof.
-  constructor; intros.
-  enough [Δ ||-<l> tEmpty ≅ tEmpty | emptyRed wfΔ] by irrelevance.
+  constructor; intros ; cbn.
+  Wirrelevance0 ; [reflexivity | eapply EqLogtoW].
+  enough [Δ ||-<l> tEmpty ≅ tEmpty | emptyRed wfΔ]< wl' > by irrelevance.
   constructor; cbn; eapply redtywf_refl; gen_typing.
+  Unshelve.
+  2: exact (emptyRed wfΔ).
+  assumption.
 Qed.
 
 (* TODO: also appears in Nat.v, should probably be more central *)
-Lemma redUOne {Γ} : [|- Γ] -> [Γ ||-U<one> U].
+Lemma redUOne {wl Γ} : [|- Γ]< wl > -> [Γ ||-U<one> U]< wl >.
 Proof.
   intros ; econstructor; [easy| gen_typing|eapply redtywf_refl; gen_typing].
 Defined.
 
-Lemma emptyTermRed {Δ} (wfΔ : [|-Δ]) : [Δ ||-<one> tEmpty : U | LRU_ (redUOne wfΔ)].
+Lemma emptyTermRed {wl Δ} (wfΔ : [|-Δ]< wl >) : [Δ ||-<one> tEmpty : U | LRU_ (redUOne wfΔ)]< wl >.
 Proof.
   econstructor.
   + eapply redtmwf_refl; gen_typing.
@@ -47,14 +54,18 @@ Proof.
   + now eapply (emptyRed (l:= zero)).
 Defined.
 
-Lemma emptyTermValid {Γ} (VΓ : [||-v Γ]):  [Γ ||-v<one> tEmpty : U | VΓ | UValid VΓ].
+Lemma emptyTermValid {wl Γ} (VΓ : [||-v Γ]< wl >):  [Γ ||-v<one> tEmpty : U | VΓ | UValid VΓ]< wl >.
 Proof.
   constructor; intros.
-  - eapply emptyTermRed. 
-  - eexists (emptyTermRed wfΔ) (emptyTermRed wfΔ) (emptyRed wfΔ); cbn.
-    + gen_typing.
-    + now eapply (emptyRed (l:=zero)).
-    + constructor; eapply redtywf_refl; gen_typing.
+  - exists (leaf _) ; intros.
+    now eapply emptyTermRed. 
+  - exists (leaf _) ; intros.
+    eexists (emptyTermRed _) (emptyTermRed _) (emptyRed _); cbn.
+    + eapply convtm_Ltrans ; [eassumption | now gen_typing].
+    + now eapply (emptyRed (l:=zero)), wfc_Ltrans.
+    + constructor; eapply redtywf_refl, wft_Ltrans ; [eassumption | ].
+      now gen_typing.
+      Unshelve. now eapply wfc_Ltrans.
 Qed.
 
 
@@ -74,43 +85,43 @@ Qed.
 Lemma liftSubst_singleSubst_eq {t u v: term} : t[u]⇑[v..] = t[u[v..]..].
 Proof. now bsimpl. Qed.
 
-Definition emptyElim {Γ A} (P : term) {n} (NA : [Γ ||-Empty A]) (p : EmptyProp Γ n) : term.
+Definition emptyElim {wl Γ A} (P : term) {n} (NA : [Γ ||-Empty A]< wl >) (p : EmptyProp (k := wl) Γ n) : term.
 Proof.
   destruct p.
   - exact (tEmptyElim P ne).
 Defined.
 
 Section EmptyElimRed.
-  Context {Γ l P}
-    (wfΓ : [|- Γ])
-    (NN : [Γ ||-Empty tEmpty])
+  Context {wl Γ l P}
+    (wfΓ : [|- Γ]< wl >)
+    (NN : [Γ ||-Empty tEmpty]< wl >)
     (RN := LREmpty_ _ NN)
-    (RP : [Γ,, tEmpty ||-<l> P])
-    (RPpt : forall n, [Γ ||-<l> n : _ | RN] -> [Γ ||-<l> P[n..]])
-    (RPext : forall n n' (Rn : [Γ ||-<l> n : _ | RN]),
-      [Γ ||-<l> n' : _ | RN] ->
-      [Γ ||-<l> n ≅ n' : _ | RN] ->
-      [Γ ||-<l> P[n..] ≅ P[n'..] | RPpt _ Rn]).
+    (RP : [Γ,, tEmpty ||-<l> P]< wl >)
+    (RPpt : forall n, [Γ ||-<l> n : _ | RN]< wl > -> W[Γ ||-<l> P[n..]]< wl >)
+    (RPext : forall n n' (Rn : [Γ ||-<l> n : _ | RN]< wl >),
+      [Γ ||-<l> n' : _ | RN]< wl > ->
+      [Γ ||-<l> n ≅ n' : _ | RN]< wl > ->
+      W[Γ ||-<l> P[n..] ≅ P[n'..] | RPpt _ Rn]< wl >).
 
   Definition emptyRedElimStmt :=
-    (forall n (Rn : [Γ ||-<l> n : _ | RN]), 
-      [Γ ||-<l> tEmptyElim P n : _ | RPpt _ Rn ] ×
-      [Γ ||-<l> tEmptyElim P n ≅ tEmptyElim P (EmptyRedTm.nf Rn) : _ | RPpt _ Rn]) ×
-    (forall n (Nn : EmptyProp Γ n) (Rn : [Γ ||-<l> n : _ | RN]), 
-      [Γ ||-<l> tEmptyElim P n : P[n..] | RPpt _ Rn ] ×
-      [Γ ||-<l> tEmptyElim P n ≅ emptyElim P NN Nn : _ | RPpt _ Rn]).
+    (forall n (Rn : [Γ ||-<l> n : _ | RN]< wl >), 
+      W[Γ ||-<l> tEmptyElim P n : _ | RPpt _ Rn ]< wl > ×
+      W[Γ ||-<l> tEmptyElim P n ≅ tEmptyElim P (EmptyRedTm.nf Rn) : _ | RPpt _ Rn]< wl >) ×
+    (forall n (Nn : EmptyProp Γ n) (Rn : [Γ ||-<l> n : _ | RN]< wl >), 
+      W[Γ ||-<l> tEmptyElim P n : P[n..] | RPpt _ Rn ]< wl > ×
+      W[Γ ||-<l> tEmptyElim P n ≅ emptyElim P NN Nn : _ | RPpt _ Rn]< wl >).
 
   Lemma emptyElimRedAux : emptyRedElimStmt.
   Proof.
     escape.
     apply EmptyRedInduction.
     - intros ? nf red ? nfprop ih.
-      assert [Γ ||-<l> nf : _ | RN]. 1:{
+      assert [Γ ||-<l> nf : _ | RN]< wl >. 1:{
         econstructor; tea.
         eapply redtmwf_refl; gen_typing.
       }
-      eapply redSubstTerm.
-      + eapply LRTmRedConv. 
+      eapply WredSubstTerm.
+      + eapply WLRTmRedConv. 
         2: unshelve eapply ih; tea.
         eapply RPext. 
         2: eapply LRTmEqSym.
@@ -118,8 +129,8 @@ Section EmptyElimRed.
       + eapply redtm_emptyelim; tea.
         cbn; gen_typing.
     - intros ? [] ?.
-      apply reflect.
-      + apply completeness.
+      apply Wreflect.
+      + apply Wcompleteness.
       + now eapply ty_emptyElim.
       + now eapply ty_emptyElim.
       + eapply convneu_emptyElim; tea.
@@ -127,66 +138,66 @@ Section EmptyElimRed.
     Unshelve. all: tea.
   Qed.
 
-  Lemma emptyElimRed : forall n (Rn : [Γ ||-<l> n : _ | RN]), [Γ ||-<l> tEmptyElim P n : _ | RPpt _ Rn ].
+  Lemma emptyElimRed : forall n (Rn : [Γ ||-<l> n : _ | RN]< wl >), W[Γ ||-<l> tEmptyElim P n : _ | RPpt _ Rn ]< wl >.
   Proof. intros. apply (fst emptyElimRedAux). Qed.
 End EmptyElimRed.
 
 
 Section EmptyElimRedEq.
-  Context {Γ l P Q}
-    (wfΓ : [|- Γ])
-    (NN : [Γ ||-Empty tEmpty])
+  Context {wl Γ l P Q}
+    (wfΓ : [|- Γ]< wl >)
+    (NN : [Γ ||-Empty tEmpty]< wl >)
     (RN := LREmpty_ _ NN)
-    (RP : [Γ,, tEmpty ||-<l> P])
-    (RQ : [Γ,, tEmpty ||-<l> Q])
-    (eqPQ : [Γ,, tEmpty |- P ≅ Q])
-    (RPpt : forall n, [Γ ||-<l> n : _ | RN] -> [Γ ||-<l> P[n..]])
-    (RQpt : forall n, [Γ ||-<l> n : _ | RN] -> [Γ ||-<l> Q[n..]])
-    (RPQext : forall n n' (Rn : [Γ ||-<l> n : _ | RN]),
-      [Γ ||-<l> n' : _ | RN] ->
-      [Γ ||-<l> n ≅ n' : _ | RN] ->
-      [Γ ||-<l> P[n..] ≅ Q[n'..] | RPpt _ Rn]).    
+    (RP : [Γ,, tEmpty ||-<l> P]< wl >)
+    (RQ : [Γ,, tEmpty ||-<l> Q]< wl >)
+    (eqPQ : [Γ,, tEmpty |- P ≅ Q]< wl >)
+    (RPpt : forall n, [Γ ||-<l> n : _ | RN]< wl > -> W[Γ ||-<l> P[n..]]< wl >)
+    (RQpt : forall n, [Γ ||-<l> n : _ | RN]< wl > -> W[Γ ||-<l> Q[n..]]< wl >)
+    (RPQext : forall n n' (Rn : [Γ ||-<l> n : _ | RN]< wl >),
+      [Γ ||-<l> n' : _ | RN]< wl > ->
+      [Γ ||-<l> n ≅ n' : _ | RN]< wl > ->
+      W[Γ ||-<l> P[n..] ≅ Q[n'..] | RPpt _ Rn]< wl >).    
 
-  Lemma RPext : forall n n' (Rn : [Γ ||-<l> n : _ | RN]),
-      [Γ ||-<l> n' : _ | RN] ->
-      [Γ ||-<l> n ≅ n' : _ | RN] ->
-      [Γ ||-<l> P[n..] ≅ P[n'..] | RPpt _ Rn].
+  Lemma RPext : forall n n' (Rn : [Γ ||-<l> n : _ | RN]< wl >),
+      [Γ ||-<l> n' : _ | RN]< wl > ->
+      [Γ ||-<l> n ≅ n' : _ | RN]< wl > ->
+      W[Γ ||-<l> P[n..] ≅ P[n'..] | RPpt _ Rn]< wl >.
   Proof.
-    intros. eapply transEq; [| eapply LRTyEqSym ]; eapply RPQext; cycle 1; tea.
+    intros. eapply WtransEq; [| eapply WLRTyEqSym ]; eapply RPQext; cycle 1; tea.
     now eapply reflLRTmEq.
     Unshelve. 2,3: eauto.
   Qed.
 
-  Lemma emptyElimRedAuxLeft : @emptyRedElimStmt _ _ P NN RPpt.
+  Lemma emptyElimRedAuxLeft : @emptyRedElimStmt _ _ _ P NN RPpt.
   Proof.
     eapply emptyElimRedAux; tea.
     + eapply RPext.
   Qed.
 
-  Lemma emptyElimRedAuxRight : @emptyRedElimStmt _ _ Q NN RQpt.
+  Lemma emptyElimRedAuxRight : @emptyRedElimStmt _ _ _ Q NN RQpt.
   Proof.
     eapply emptyElimRedAux; tea.
-    + intros. eapply transEq; [eapply LRTyEqSym |]; eapply RPQext; cycle 1; tea.
+    + intros. eapply WtransEq; [eapply WLRTyEqSym |]; eapply RPQext; cycle 1; tea.
       now eapply reflLRTmEq.
     Unshelve. all:tea.
   Qed.
 
   Lemma emptyElimRedEqAux :
-    (forall n n' (Rnn' : [Γ ||-<l> n ≅ n' : _ | RN]) (Rn : [Γ ||-<l> n : _ | RN]) (Rn' : [Γ ||-<l> n' : _ | RN]),
-      [Γ ||-<l> tEmptyElim P n ≅ tEmptyElim Q n' : _ | RPpt _ Rn ]) ×
-    (forall n n' (Rnn' : EmptyPropEq Γ n n') (Rn : [Γ ||-<l> n : _ | RN]) (Rn' : [Γ ||-<l> n' : _ | RN]),
-      [Γ ||-<l> tEmptyElim P n ≅ tEmptyElim Q n' : _ | RPpt _ Rn ]).
+    (forall n n' (Rnn' : [Γ ||-<l> n ≅ n' : _ | RN]< wl >) (Rn : [Γ ||-<l> n : _ | RN]< wl >) (Rn' : [Γ ||-<l> n' : _ | RN]< wl >),
+      W[Γ ||-<l> tEmptyElim P n ≅ tEmptyElim Q n' : _ | RPpt _ Rn ]< wl >) ×
+    (forall n n' (Rnn' : EmptyPropEq wl Γ n n') (Rn : [Γ ||-<l> n : _ | RN]< wl >) (Rn' : [Γ ||-<l> n' : _ | RN]< wl >),
+      W[Γ ||-<l> tEmptyElim P n ≅ tEmptyElim Q n' : _ | RPpt _ Rn ]< wl >).
   Proof.
     apply EmptyRedEqInduction.
     - intros ?? nfL nfR redL redR ? prop ih RL RR; edestruct @EmptyPropEq_whnf; eauto. 
-      assert [Γ ||-<l> nfL : _ | RN] by (eapply redTmFwd; cycle 1; tea).
-      assert [Γ ||-<l> nfR : _ | RN] by (eapply redTmFwd; cycle 1; tea).
-      eapply LREqTermHelper.
+      assert [Γ ||-<l> nfL : _ | RN]< wl > by (eapply redTmFwd; cycle 1; tea).
+      assert [Γ ||-<l> nfR : _ | RN]< wl > by (eapply redTmFwd; cycle 1; tea).
+      eapply WLREqTermHelper.
       * eapply (fst emptyElimRedAuxLeft).
       * eapply (fst emptyElimRedAuxRight).
       * eapply RPQext. 1: tea.
         now econstructor.
-      * eapply LRTmEqRedConv.
+      * eapply WLRTmEqRedConv.
         + eapply RPext; tea. 
           eapply LRTmEqSym; eapply redwfSubstTerm; cycle 1; tea.
         + unshelve erewrite (redtmwf_det _ _ (EmptyRedTm.red RL) redL); tea.
@@ -196,14 +207,14 @@ Section EmptyElimRedEq.
           now eapply ih.
         Unshelve. tea. 2, 4: tea. 
     - intros ?? neueq ??. escape. inversion neueq.
-      assert [Γ |- P[ne..] ≅ Q[ne'..]]. 1:{
-        eapply escapeEq. eapply RPQext; tea.
+      assert [Γ |- P[ne..] ≅ Q[ne'..]]< wl >. 1:{
+        eapply WescapeEq. eapply RPQext; tea.
         econstructor.
         1,2: now eapply redtmwf_refl.
         2: now constructor.
         gen_typing.
       }
-      eapply neuTermEq.
+      eapply WneuTermEq.
       + eapply ty_emptyElim; tea.
       + eapply ty_conv. 
         1: eapply ty_emptyElim; tea.
@@ -213,109 +224,168 @@ Section EmptyElimRedEq.
   Qed.
 
   Lemma emptyElimRedEq :
-    (forall n n' (Rnn' : [Γ ||-<l> n ≅ n' : _ | RN]) (Rn : [Γ ||-<l> n : _ | RN]) (Rn' : [Γ ||-<l> n' : _ | RN]), 
-      [Γ ||-<l> tEmptyElim P n ≅ tEmptyElim Q n' : _ | RPpt _ Rn ]).
+    (forall n n' (Rnn' : [Γ ||-<l> n ≅ n' : _ | RN]< wl >) (Rn : [Γ ||-<l> n : _ | RN]< wl >) (Rn' : [Γ ||-<l> n' : _ | RN]< wl >), 
+      W[Γ ||-<l> tEmptyElim P n ≅ tEmptyElim Q n' : _ | RPpt _ Rn ]< wl >).
   Proof. apply emptyElimRedEqAux. Qed.
 End EmptyElimRedEq.
 
 
 
 Section EmptyElimValid.
-  Context {Γ l P}
-    (VΓ : [||-v Γ])
+  Context {wl Γ l P}
+    (VΓ : [||-v Γ]< wl >)
     (VN := emptyValid (l:=l) VΓ)
-    (VΓN := validSnoc VΓ VN)
-    (VP : [Γ ,, tEmpty ||-v<l> P | VΓN]).
+    (VΓN := validSnoc' VΓ VN)
+    (VP : [Γ ,, tEmpty ||-v<l> P | VΓN]< wl >).
   
 
   Lemma emptyElimValid {n}
-    (Vn : [Γ ||-v<l> n : tEmpty | VΓ | VN])
+    (Vn : [Γ ||-v<l> n : tEmpty | VΓ | VN]< wl >)
     (VPn := substS VP Vn)
-    : [Γ ||-v<l> tEmptyElim P n : _ | VΓ | VPn].
+    : [Γ ||-v<l> tEmptyElim P n : _ | VΓ | VPn]< wl >.
   Proof.
     constructor; intros.
     - instValid Vσ; cbn.
-      irrelevance0.  1: now rewrite singleSubstComm'.
       epose proof (Vuσ := liftSubstS' VN Vσ).
-      instValid Vuσ; escape.
+      instValid Vuσ; escape ; Wescape.
+      unshelve eapply TreeTmSplit.
+      1: do 2 eapply DTree_fusion ; shelve.
+      intros wl'' Ho HA.
+      pose (f' := over_tree_le Ho).
+      Wirrelevance0.  1: now rewrite singleSubstComm'.
       unshelve eapply emptyElimRed; tea.
-      + intros m Rm.
+      + econstructor ; eapply redtywf_refl.
+        eapply wft_term, ty_empty, wfc_Ltrans ; eassumption.
+      + intros m Rm ; cbn in *.
         rewrite up_single_subst. 
-        unshelve eapply validTy; cycle 1; tea.
-        unshelve econstructor; [now bsimpl| now cbn].
+        unshelve eapply validTy.
+        6 : eassumption.
+        1: now eapply wfLCon_le_trans.
+        1: now eapply wfc_Ltrans.
+        unshelve econstructor; [| cbn ; now eapply TmLogtoW].
+        now eapply subst_Ltrans.
+      + irrelevanceRefl.
+        eapply RVn, over_tree_fusion_l, over_tree_fusion_l ; exact Ho.
+      + eapply RVP, over_tree_fusion_r, over_tree_fusion_l ; exact Ho.
       + intros m m' Rm Rm' Rmm'; cbn.
-        irrelevance0. 1: now rewrite up_single_subst.
+        Wirrelevance0. 1: now rewrite up_single_subst.
         rewrite up_single_subst.
-        unshelve eapply validTyExt; cycle 1 ; tea.
-        1,2: unshelve econstructor; [now bsimpl| now cbn].
-        unshelve econstructor; [|now cbn].
-        bsimpl; cbn; eapply reflSubst.
+        unshelve eapply validTyExt; cycle 3 ; tea.
+        1: now eapply wfLCon_le_trans.
+        1: now eapply wfc_Ltrans.
+        1,2: unshelve econstructor; [now eapply subst_Ltrans | now eapply TmLogtoW].
+        unshelve econstructor; [|cbn ; now eapply TmEqLogtoW].
+        eapply eqsubst_Ltrans.
+        bsimpl; cbn; now eapply reflSubst.
+        Unshelve.
+        3: eapply  over_tree_fusion_l, over_tree_fusion_r ; exact Ho.
+        now constructor.
     - instAllValid Vσ Vσ' Vσσ'.
-      irrelevance0.  1: now rewrite singleSubstComm'.
       pose (Vuσ := liftSubstS' VN Vσ).
       pose proof (Vuσ' := liftSubstS' VN Vσ').
       pose proof (Vuσrea :=  liftSubstSrealign' VN Vσσ' Vσ').
       pose proof (Vuσσ' := liftSubstSEq' VN Vσσ').
-      instValid Vuσ'; instAllValid Vuσ Vuσrea Vuσσ'; escape.
+      instValid Vuσ'; instAllValid Vuσ Vuσrea Vuσσ'; escape ; Wescape.
+      unshelve eapply TreeTmEqSplit.
+      1: do 2 eapply DTree_fusion ; [ .. | eapply DTree_fusion] ; shelve.
+      intros wl'' Ho HA.
+      pose (f' := over_tree_le Ho).
+      Wirrelevance0.  1: now rewrite singleSubstComm'.
       unshelve eapply emptyElimRedEq; tea; fold subst_term.
-      all: try now (irrelevance; now rewrite elimSuccHypTy_subst).
+      + econstructor ; eapply redtywf_refl.
+        eapply wft_term, ty_empty, wfc_Ltrans ; eassumption.
       + intros m Rm.
         rewrite up_single_subst. 
-        unshelve eapply validTy; cycle 1; tea.
-        unshelve econstructor; [now bsimpl| now cbn].
+        unshelve eapply validTy; cycle 5; tea.
+        1: unshelve econstructor; [now eapply subst_Ltrans | now eapply TmLogtoW].
+      + irrelevanceRefl.
+        eapply RVn, over_tree_fusion_l, over_tree_fusion_l ; exact Ho.
+      + eapply RVP0, over_tree_fusion_r, over_tree_fusion_l ; exact Ho.
+      + eapply RVP, over_tree_fusion_l, over_tree_fusion_r ; exact Ho.
+      + now eapply convty_Ltrans.
       + intros m Rm.
         rewrite up_single_subst. 
-        unshelve eapply validTy; cycle 1; tea.
-        unshelve econstructor; [now bsimpl| now cbn].
+        unshelve eapply validTy; cycle 5; tea.
+        1: unshelve econstructor; [now eapply subst_Ltrans | now eapply TmLogtoW].
       + intros m m' Rm Rm' Rmm'; cbn.
-        irrelevance0. 1: now rewrite up_single_subst.
+        Wirrelevance0. 1: now rewrite up_single_subst.
         rewrite up_single_subst.
-        unshelve eapply validTyExt; cycle 1 ; tea.
-        1,2: unshelve econstructor; [now bsimpl| now cbn].
-        unshelve econstructor; [|now cbn].
-        now bsimpl.
+        unshelve eapply validTyExt ;cycle 6.
+        7: eassumption.
+        1,2: unshelve econstructor; [now eapply subst_Ltrans | now eapply TmLogtoW].
+        1: unshelve econstructor; [|cbn ; now eapply TmEqLogtoW].
+        1: now eapply eqsubst_Ltrans.
+      + irrelevanceRefl ; eapply REVn.
+        eapply over_tree_fusion_l, over_tree_fusion_r, over_tree_fusion_r ; exact Ho.
+      + irrelevanceRefl ; eapply RVn0.
+        eapply over_tree_fusion_r, over_tree_fusion_r, over_tree_fusion_r ; exact Ho.
+        Unshelve.
+        all: try eassumption.
   Qed.
-
 End EmptyElimValid.
 
-Lemma emptyElimCongValid {Γ l P Q n n'}
-    (VΓ : [||-v Γ])
+Lemma emptyElimCongValid {wl Γ l P Q n n'}
+    (VΓ : [||-v Γ]< wl >)
     (VN := emptyValid (l:=l) VΓ)
-    (VΓN := validSnoc VΓ VN)
-    (VP : [Γ ,, tEmpty ||-v<l> P | VΓN])
-    (VQ : [Γ ,, tEmpty ||-v<l> Q | VΓN])
-    (VPQ : [Γ ,, tEmpty ||-v<l> P ≅ Q | VΓN | VP])
-    (Vn : [Γ ||-v<l> n : _ | VΓ | VN])
-    (Vn' : [Γ ||-v<l> n' : _ | VΓ | VN])
-    (Veqn : [Γ ||-v<l> n ≅ n' : _ | VΓ | VN])
+    (VΓN := validSnoc' VΓ VN)
+    (VP : [Γ ,, tEmpty ||-v<l> P | VΓN]< wl >)
+    (VQ : [Γ ,, tEmpty ||-v<l> Q | VΓN]< wl >)
+    (VPQ : [Γ ,, tEmpty ||-v<l> P ≅ Q | VΓN | VP]< wl >)
+    (Vn : [Γ ||-v<l> n : _ | VΓ | VN]< wl >)
+    (Vn' : [Γ ||-v<l> n' : _ | VΓ | VN]< wl >)
+    (Veqn : [Γ ||-v<l> n ≅ n' : _ | VΓ | VN]< wl >)
     (VPn := substS VP Vn) :
-    [Γ ||-v<l> tEmptyElim P n ≅ tEmptyElim Q n' : _ | VΓ | VPn].
+    [Γ ||-v<l> tEmptyElim P n ≅ tEmptyElim Q n' : _ | VΓ | VPn]< wl >.
 Proof.
   constructor; intros.
   pose (Vuσ := liftSubstS' VN Vσ).
-  instValid Vσ; instValid Vuσ; escape.
-  irrelevance0.  1: now rewrite singleSubstComm'.
+  instValid Vσ; instValid Vuσ; escape ; Wescape.
+  unshelve eapply TreeTmEqSplit.
+  1: do 2 eapply DTree_fusion ; [ .. | eapply DTree_fusion | eapply DTree_fusion] ; shelve.
+  intros wl'' Ho HA.
+  pose proof (f':= over_tree_le Ho).
+  Wirrelevance0.  1: now rewrite singleSubstComm'.
   unshelve eapply emptyElimRedEq; tea; fold subst_term.
-  all: try (irrelevance; now rewrite elimSuccHypTy_subst).
-  + intros m Rm.
+  - unshelve econstructor.
+    eapply redtywf_refl, wft_term, ty_empty.
+    now eapply wfc_Ltrans.
+  - intros m Rm.
     rewrite up_single_subst. 
-    unshelve eapply validTy; cycle 1; tea.
-    unshelve econstructor; [now bsimpl| now cbn].
-  + intros m Rm.
+    unshelve eapply validTy; cycle 4; tea.
+    + now eapply wfc_Ltrans.
+    + unshelve econstructor; [ | now eapply TmLogtoW].
+      now eapply subst_Ltrans.
+  - irrelevanceRefl ; eapply RVn.
+    eapply over_tree_fusion_l, over_tree_fusion_l, over_tree_fusion_r ; exact Ho.
+  - eapply RVP, over_tree_fusion_l, over_tree_fusion_l ; exact Ho.
+  - eapply RVQ, over_tree_fusion_r, over_tree_fusion_l ; exact Ho.
+  - now eapply convty_Ltrans.
+  - intros m Rm ; cbn in *.
     rewrite up_single_subst. 
-    unshelve eapply validTy; cycle 1; tea.
-    unshelve econstructor; [now bsimpl| now cbn].
-  + intros m m' Rm Rm' Rmm'; cbn.
-    irrelevance0. 1: now rewrite up_single_subst.
+    unshelve eapply validTy; cycle 4; tea.
+    + now eapply wfc_Ltrans.
+    + unshelve econstructor; [ | now eapply TmLogtoW].
+      now eapply subst_Ltrans.
+  - intros m m' Rm Rm' Rmm'; cbn.
+    Wirrelevance0. 1: now rewrite up_single_subst.
     rewrite up_single_subst.
-    eapply transEq; cycle 1.
-    - unshelve eapply validTyEq. 
-      7: tea. 1: tea.
-      unshelve econstructor; [now bsimpl| now cbn].
-    - unshelve eapply validTyExt; cycle 1 ; tea.
-    1,2: unshelve econstructor; [now bsimpl| now cbn].
-    unshelve econstructor; [|now cbn].
-    bsimpl. eapply reflSubst.
+    eapply WtransEq; cycle 1.
+    + unshelve eapply validTyEq. 
+      9: eassumption.
+      3: unshelve econstructor; [ | now eapply TmLogtoW].
+      2: now eapply subst_Ltrans.
+    + unshelve eapply validTyExt; cycle 3 ; tea.
+      3: unshelve econstructor; [ now eapply subst_Ltrans | now eapply TmLogtoW].
+      1: unshelve econstructor; [ now eapply subst_Ltrans | now eapply TmLogtoW].
+      1: unshelve econstructor; [ eapply eqsubst_Ltrans | now eapply TmEqLogtoW].
+      bsimpl. eapply reflSubst.
+  - irrelevanceRefl ; eapply RVeqn.
+    now eapply over_tree_fusion_r, over_tree_fusion_l, over_tree_fusion_r ; exact Ho.
+  - irrelevanceRefl ; eapply RVn'.
+    now eapply over_tree_fusion_l, over_tree_fusion_r, over_tree_fusion_r ; exact Ho.
+    Unshelve.
+    2,6,7: now do 3 (eapply over_tree_fusion_r) ; exact Ho.
+    all: assumption.
 Qed.
 
 End Empty.
